src/EndToEnd.v
@@ -1,3 +1,5 @@
+Require Import List seq ssreflect ssrbool ssrnat ZArith eqtype.
+
 Require Import AbstractGen Property SetOfOutcomes.
 
 Definition semProperty (P : Pred QProp) : Prop :=
@@ -6,4 +8,27 @@ Definition semProperty (P : Pred QProp) : Prop :=
 Definition semTestable {A : Type} {_ : @Testable Pred A} (a : A) : Prop :=
   semProperty (property a).
 
-
+Lemma semForAllShrink : forall {A prop : Type} {H : Testable prop}
+    show (gen : Pred A) shrink (pf : A -> prop),
+  semProperty (@forAllShrink Pred _ _ _ H show gen shrink pf) <->
+  (forall a : A, gen a -> (semProperty (property (pf a)))).
+Proof.
+  move => A prop Htest show gen shrink pf. split => H'.
+  - move => a Hgen. simpl in H'.
+    unfold bindP, semProperty in * => qp H''.
+    move /(_ qp) : H' => H'. apply : H'.
+    exists a. split => //=.
+    unfold fmapP, bindP. exists (MkRose qp (lazy nil)).
+    split. Focus 2. compute. destruct qp as [[[? ? ? ? ? ?] []]]. reflexivity.
+    unfold promoteP.
+    exists qp. admit. (* unfold fmapRose, props. *)
+    (* this seems to need some generalization 1000 -> n + induction *)
+  - unfold semProperty in * => qp Hforall.
+    unfold forAllShrink in Hforall. rewrite bindGen_def in Hforall.
+    move : Hforall => [a [Hgen H]]. apply : H' => //=.
+    unfold shrinking in H. rewrite fmapGen_def in H.
+    move : H => [rqp [H1 H2]]. subst qp.
+    unfold promote, PredMonad, promoteP in H1.
+    move : H1 => [qp H]. subst rqp.
+    (* this is wrong ... probably the semantics of promoteP *)
+Abort.
