src/Gen.v
@@ -73,7 +73,6 @@ Proof.
 Definition sizedG {A : Type} (f : nat -> Gen A) : Gen A :=
   MkGen (fun r n => match f n with MkGen m => m r n end).
 
-(* Could this be added to the typeclass too ? It seems so*)
 Definition promoteG {M : Type -> Type} {A : Type} 
            (liftFun : (Gen A -> A) -> M (Gen A) -> M A) 
            (m : M (Gen A)) : Gen (M A) :=
